list_inst1.v
@@ -1,0 +1,463 @@
+Require Import VST.concurrency.conclib.
+From iris.algebra Require Import excl auth gmap agree gset.
+Require Import flows.inset_flows.
+Require Import flows.auth_ext.
+Require Import flows.multiset_flows.
+Require Import flows.flows.
+Require Import iris_ora.algebra.gmap.
+Require Import iris_ora.logic.own.
+Require Import iris_ora.algebra.ext_order.
+Require Import iris_ora.algebra.frac_auth.
+Require Import VST.floyd.proofauto.
+Require Import VST.atomics.general_locks.
+Require Import VST.floyd.library.
+Require Import VST.atomics.verif_lock_atomic.
+Require Import tmpl.puretree.
+Require Import tmpl.list. (*binary search tree*)
+Require Import tmpl.keyset_ra_ora.
+Require Import tmpl.puretree.
+Require Import tmpl.data_struct.
+Require Import tmpl.flows_ora.
+
+
+#[export] Instance CompSpecs : compspecs. make_compspecs prog. Defined.
+Definition Vprog : varspecs.  mk_varspecs prog. Defined.
+
+#[global] Instance gmap_inhabited V : Inhabitant (gmap key V).
+Proof. unfold Inhabitant; apply empty. Defined.
+
+#[global] Instance number_inhabited: Inhabitant number.
+Proof. unfold Inhabitant; apply Pos_Infinity. Defined.
+
+Section give_up_traverse.
+  Context `{N: NodeRep } `{EqDecision K} `{Countable K}.
+  Context `{!cinvG Σ, atom_impl : !atomic_int_impl (Tstruct _atom_int noattr),
+            !flowintG Σ, !nodesetG Σ, !keysetG Σ, !keymapG Σ, inG Σ (frac_authR (agreeR Node))}.
+  
+
+(* struct node {int key; void *value; struct tree_t *left, *right;} node;*)
+Definition t_struct_list := Tstruct _node noattr.
+(* Define for dynamic list *)
+Definition struct_dlist := Tstruct _DList noattr.
+
+(* struct tree_t {node *t; lock_t *lock; int min; int max; } tree_t; *)
+(* Definition t_struct_tree_t := Tstruct _tree_t noattr. *)
+
+(* node_rep_R r.1.1.1 r.1.2 r.2 g, and r is type of node_info *)
+
+(*
+Class NodeRep : Type := {
+    node : val → @multiset_flowint_ur Key _ _ → gmap Key Value -> gmap nat Node -> mpred;
+    (* node_sep_star: ∀ n I_n I_n' C C', node n I_n C ∗ node n I_n' C' -∗ False; *)
+    node_rep_R_valid_pointer: forall n I_n C next, node n I_n C next -∗ valid_pointer n;
+    node_rep_R_pointer_null: forall n I_n C next, node n I_n C next -∗ ⌜is_pointer_or_null n⌝;
+    node_size: nat;
+}.
+
+ *)
+
+Local Instance nzmap_filter: Filter (Z * nat) (@multiset_flows.K_multiset Key Z.eq_dec Z_countable).
+Proof.
+  intros ???.
+  eapply (NZMap (filter P (nzmap_car H2)) _).
+  Unshelve.
+  unfold bool_decide.
+  destruct (nzmap_wf_decision Key (filter P (nzmap_car H2))); try done.
+  unfold not in n.
+  apply n. clear n.
+  rewrite / nzmap_wf /map_Forall.
+  intros i x Hf.
+  assert (nzmap_wf (nzmap_car H2)) as wfH. { apply nzmap_is_wf. }
+  apply map_lookup_filter_Some_1_1 in Hf.
+  rewrite /nzmap_wf /map_Forall in wfH.
+  eapply wfH; eauto.
+Defined.
+
+Lemma nzmap_lookup_filter_Some `{Countable K} `{CCM A}
+  (P : Z * nat → Prop) (H7 : ∀ x : Z * nat, Decision (P x)) 
+  (m : nzmap Z nat) (i : Z) (x : nat) :
+  filter P m !! i = Some x <-> m !! i = Some x /\ P (i, x).
+Proof.
+  unfold lookup, nzmap_lookup .
+  split.
+  - intros.
+    destruct m.
+    unfold filter in H3.
+    simpl in H3.
+    apply map_lookup_filter_Some in H3. auto.
+  - intros.
+    destruct m.
+    unfold filter. simpl.
+    rewrite map_lookup_filter_Some. auto.
+Qed.
+
+Lemma nzmap_dom_filter_subseteq (P : Z * nat → Prop) `{!∀ x, Decision (P x)} (m : nzmap Z nat):
+  dom (filter P m) ⊆ dom m.
+Proof.
+  destruct m.
+  unfold filter.
+  simpl.
+  unfold nzmap_dom. simpl.
+  apply dom_filter_subseteq.
+Qed.
+
+#[local] Obligation Tactic := idtac.
+
+#[local] Program Instance my_specific_tree_rep : NodeRep := {
+  node := fun (n : Node) (In : @multiset_flowint_ur Key _ _) (C: gmap Key data_struct.Value)
+            (next:  gmap nat val) =>
+  if eq_dec n nullval
+  then ⌜∀ y : Key, ¬ in_outsets val_EqDecision Node_countable Key y In ∧
+                     ¬ ∃ n1 : Node, n1 ≠ n ∧ in_inset val_EqDecision Node_countable Key y In n1 ∧
+                     C = ∅⌝ ∧ emp
+  else
+  (∃ (x : Z) (v : val) (n' : Node),
+      ⌜and (Z.le Int.min_signed x) (Z.le x Int.max_signed) /\
+       is_pointer_or_null (next !!! 0)  /\
+          (tc_val (tptr Tvoid) v) ∧ C = {[x := v]} ∧ dom (out_map In) = {[n']} ∧
+        (forall y, in_outset _ _ Key y In n' <-> Z.lt x y ∧ in_inset _ _ Key y In n) ∧
+        (forall y, in_outsets _ _ Key y In -> in_outset _ _ Key y In n') ⌝ ∧
+       data_at Ews t_struct_list (Vint (Int.repr x), (v, (next !!! 0))) n ∗
+       malloc_token Ews t_struct_list n); node_size := 1}.
+(* ; node_rep_R_valid_pointer }. *)
+Next Obligation.
+  intros n In Cn next.
+  destruct (EqDec_val n nullval). 
+  - simpl. rewrite e. auto.
+  - rewrite if_false; auto. iIntros "H".
+    iDestruct "H" as (x v) "(%HJ & (H1 & H2))".
+    iStopProof. entailer !.
+Defined.
+Next Obligation.
+  intros n In Cn next.
+  destruct (EqDec_val n nullval).
+  - simpl. rewrite e. auto.
+  - rewrite if_false; auto.
+    iIntros "H".
+    iDestruct "H" as (x v) "(%HJ & (H1 & H2))".
+    iStopProof. entailer !.
+Defined.
+
+(* Spec of findnext function *)
+(* FOUND = 0, NOTFOUND = 1, NULLNEXT = 2 (NULLNEXT = NULL || NEXT ) *)
+Definition findnext_spec :=
+  DECLARE _findNext
+  WITH x: Z, p: Node, n: val, n_pt : val, Ip : flowintT,
+                Cp : (gmap Key data_struct.Value), nextp : gmap nat Node, sh: share, gv: globals
+  PRE [ tptr t_struct_list, tptr (tptr tvoid), tint ]
+          PROP (writable_share sh;
+                (Int.min_signed ≤ x ≤ Int.max_signed)%Z
+          (*; is_pointer_or_null pa; is_pointer_or_null pb*) )
+          PARAMS (p; n; Vint (Int.repr x)) GLOBALS (gv)
+          SEP (node p Ip Cp nextp ∗ ⌜p <> nullval /\ in_inset _ _ Key x Ip p⌝ ∧
+               (* field_at sh (t_struct_tree) [StructField _t] r.1.1.1 p; *)
+               data_at sh (tptr tvoid) n_pt n)
+  POST [ tint ]
+  ∃ (stt: enum), ∃ (n' next : val), ∃ (nnext : Node),
+         PROP (match stt with
+               | F | NF => (n' = p)
+               | NN => (n' = next)
+               end; dom (out_map Ip) = {[nnext]})
+        LOCAL (temp ret_temp (enums stt))
+        SEP (match stt with
+               | F | NF => ⌜¬in_outsets _ _ Key x Ip⌝ ∧ data_at sh (tptr tvoid) n_pt n
+               | NN => ⌜in_outset _ _ Key x Ip nnext⌝ ∧ data_at sh (tptr tvoid) next n
+             end;
+               node p Ip Cp nextp).
+
+Lemma findNext: semax_body Vprog Gprog f_findNext findnext_spec.
+Proof.
+  start_function.
+  Intros.
+  unfold node.
+  unfold my_specific_tree_rep.
+  rewrite -> if_false; eauto.
+  Intros x0 v0.
+  forward.
+  forward_if. (* if (_x < _y) *)
+  - forward. forward. forward.
+    Exists NN (nextp !!! 0) (nextp !!! 0) n'.
+    unfold node, my_specific_tree_rep.
+    rewrite -> if_false; auto.
+    Exists x0 v0 .
+    entailer !.
+    specialize (H9 x).
+    set_solver.
+    Exists n'. entailer !.
+  - (* if (_x > _y) *)
+    forward_if.
+    repeat forward.
+    Exists NF p p n'.
+    entailer !.
+    apply (H10 x), (H9 x) in H7.
+    lia.
+    rewrite /node /my_specific_tree_rep.
+    rewrite -> if_false; auto.
+    Exists x0 v0 n'. entailer !.
+    (* x = y *)
+    forward.
+    Exists F p p n'.
+    rewrite /node /my_specific_tree_rep.
+    rewrite -> if_false; auto.
+    Exists x0 v0 n'.
+    entailer !.
+    assert (x = x0). lia. subst x0.
+    apply (H10 x) in H7.
+    apply (H9 x) in H7.
+    lia.
+Qed.
+
+Definition surely_malloc_spec :=
+  DECLARE _surely_malloc
+   WITH t: type, gv: globals
+   PRE [ size_t ]
+       PROP (and (Z.le 0 (sizeof t)) (Z.lt (sizeof t) Int.max_unsigned);
+                complete_legal_cosu_type t = true;
+                natural_aligned natural_alignment t = true)
+       PARAMS (Vptrofs (Ptrofs.repr (sizeof t))) GLOBALS (gv)
+       SEP (mem_mgr gv)
+    POST [ tptr tvoid ]
+    ∃ p: _,
+       PROP ()
+       RETURN (p)
+       SEP (mem_mgr gv; malloc_token Ews t p; data_at_ Ews t p).
+
+Fixpoint list_to_gmap_aux (l : list Node) (key : nat) : gmap nat Node :=
+  match l with
+  | [] => ∅
+  | x :: xs => <[key:=x]> (list_to_gmap_aux xs (S key))
+  end.
+
+Definition list_to_gmap (l : list Node) : gmap nat Node :=
+  list_to_gmap_aux l 0.
+
+(*  Ip : @flowintT _ K_multiset_ccm  _ _ *)
+
+Check contextualLeq _ .
+(*  @flows.int (@multiset_flows.K_multiset Key Z.eq_dec Z_countable) K_multiset_ccm _  _
+          {|infR := {[ tp := S ]}; outR := <<[ Znth 0 next0 := S ]>> ∅ |} = Ip; *)
+
+Definition flow_int I:= @flows.int (@multiset_flows.K_multiset Key Z.eq_dec Z_countable)
+                           K_multiset_ccm _ _ I.
+
+Definition remap_out I tp new_node := flow_int {| infR := inf_map I; outR := <<[ tp := 0%CCM]>> <<[ new_node := out I tp ]>>(out_map I) |}.
+
+Definition insertOp_spec :=
+  DECLARE _insertOp
+    WITH x: Z, v: val, stt: Z, p: Node, tp: val, l: val, dl: val, Ip: flowintT,
+         Cp: (gmap Key data_struct.Value), next0: list Node, next: list Node, sh: share, gv: globals
+  PRE [ tptr (tptr t_struct_list), tint, tptr tvoid, tint, tptr (struct_dlist)]
+  PROP (repable_signed x; is_pointer_or_null v; length next = node_size;
+        in_inset _ _ Key x Ip tp; ¬ in_outsets _ _ Key x Ip;
+        is_pointer_or_null (Znth 0 next) (* ; tp = nullval*) )
+  PARAMS (p; Vint (Int.repr x); v; Vint (Int.repr stt); l)
+  GLOBALS (gv)
+  SEP (mem_mgr gv;
+       node tp Ip Cp (list_to_gmap next0);
+       field_at Tsh (struct_dlist) (DOT _list) dl l;
+       data_at Ews (tptr t_struct_list) tp p;
+       data_at Ews (tarray (tptr tvoid) (Zlength next)) next dl)
+  POST[ tvoid ]
+  ∃ (new_node : Node) (I_new I1: flowintT),
+  PROP (new_node <> nullval)
+  LOCAL ()
+  SEP (mem_mgr gv; node new_node I_new ({[x := v]}) (list_to_gmap next);
+       node tp I1 Cp (list_to_gmap next0);
+       field_at Tsh struct_dlist (DOT _list) dl l;
+       data_at Ews (tptr t_struct_list) new_node p;
+     data_at Ews (tarray (tptr tvoid) (Zlength next)) next dl;
+     ⌜∀ I0, contextualLeq _ (I0 ⋅ Ip) ((remap_out Ip tp new_node) ⋅ I1 ⋅ I_new) ∧
+                inf ((remap_out Ip tp new_node) ⋅ I1 ⋅ I_new) new_node = 0%CCM⌝).
+
+Search data_at.
+
+(*
+Lemma ne_pointer sh p1 p2 t v1 v2:
+  writable_share sh -> sh ≠ Share.bot -> (0 < sizeof t)%Z ->
+  data_at sh t v1 p1 ∗ data_at sh t v2 p2 -∗ ⌜p1 <> p2⌝.
+Proof.
+  intros.
+  iIntros "(H1 & H2)".
+  destruct (decide (p1 = p2)) as [-> | Hp]; try done.
+  iDestruct (data_at_conflict with "[$H1 $H2]") as "H"; try done.
+Qed.
+*)
+
+Definition Gprog : funspecs :=
+    ltac:(with_library prog [acquire_spec; release_spec; makelock_spec; surely_malloc_spec; insertOp_spec]).
+
+(* Proving insertOp satisfies spec *)
+Lemma insertOp: semax_body Vprog Gprog f_insertOp insertOp_spec.
+Proof.
+  start_function.
+  forward_call (t_struct_list, gv).
+  unfold node, my_specific_tree_rep.
+  Intros new_node.
+  destruct (decide (tp = nullval)) as [Heq | Hneq].
+  {
+    rewrite Heq.
+    rewrite -> if_true; auto.
+    Intros.
+    forward. forward. forward. forward. entailer !. rewrite Zlength_correct.
+    simpl in *. rewrite -> H3. lia.
+    specialize (H7 x).
+    destruct H7.
+    
+    
+  assert (tp <> nullval). admit.
+  rewrite -> if_false; auto.
+  Intros x0 v0.
+  forward. forward. forward. forward.
+  rewrite Zlength_correct.
+  simpl in *.
+  rewrite -> H3.
+  entailer !.
+  Intros n'.
+  forward. forward.
+  assert_PROP (new_node <> tp). entailer !.
+  unfold in_outsets in H5.
+  assert (forall n, ¬ in_outset val_EqDecision Node_countable Key x Ip n) as allNot. set_solver.
+  assert (Z.le x x0) as Hle.
+  { apply Ztac.elim_concl_le.
+    intros Hlt.
+    assert (Z.lt x0 x ∧ in_inset val_EqDecision Node_countable Key x Ip tp) as Hcm; auto.
+    apply (H13 x) in Hcm. set_solver.
+  }
+  assert_PROP (new_node <> nullval). entailer !.
+  assert (list_to_gmap_aux next 0 !!! 0 = Znth 0 next /\
+            list_to_gmap_aux next0 0 !!! 0 = Znth 0 next0) as (Hznth & Hznth0).
+  { split; unfold Znth; [destruct next as [| x' xs'] | destruct next0 as [| x' xs']];
+      simpl; auto; rewrite lookup_total_insert; auto.
+  }
+  rewrite /in_outset /out /in_inset in H13.
+  rewrite /in_outsets /in_outset /out in H14.
+  rewrite /in_outset in allNot.
+   
+  Exists new_node.
+  set m1 := filter (fun '(k, _) => Z.lt x k) (inf Ip tp).
+  (* Set Printing Implicit. *)
+  Exists (flow_int {| infR := {[ new_node := inf Ip tp ]}; outR := <<[ tp := m1 ]>> ∅ |}).
+  Exists (flow_int {| infR := {[ tp := m1 ]}; outR := <<[ n' := out Ip n' ]>> ∅ |}).
+  rewrite / node / my_specific_tree_rep.
+  rewrite if_false; auto.
+  rewrite if_false; auto.
+  entailer !.
+  Exists x v tp.
+  Exists x0 v0 n'.
+  entailer !.
+  repeat split; try done.
+  - rewrite /list_to_gmap Hznth; auto. 
+  - rewrite / out_map /inf /=.
+    rewrite <- leibniz_equiv_iff.
+    rewrite nzmap_dom_insert_nonzero. set_solver.
+    rewrite /in_inset in H4.
+    apply nzmap_elem_of_dom_total in H4.
+    destruct (lookup) eqn: Eqn.
+    rewrite /inf Eqn /= in H4.
+    rewrite <- nzmap_elem_of_dom_total in H4.
+    admit.
+    unfold inf in H4. rewrite Eqn in H4. simpl in H4.
+    contradiction.
+  - rewrite /in_outset /out /out_map //= nzmap_lookup_total_insert in H11.
+    rewrite / in_inset in H4.
+    apply nzmap_elem_of_dom_total in H11.
+    rewrite nzmap_lookup_total_alt in H11.
+    rewrite /default /id in H11.
+    destruct (lookup) eqn: Eqn.
+    apply (nzmap_lookup_filter_Some (λ '(k, _), (x < k)%Z) _ (@inf (@multiset_flows.K_multiset Key Z.eq_dec Z_countable)
+            (@multiset_flows.K_multiset_ccm Key Z.eq_dec Z_countable) val_EqDecision Node_countable Ip
+            tp)  y n) in Eqn.
+    lia.
+    contradiction.
+  - rewrite /in_outset /out /out_map /= nzmap_lookup_total_insert /inf in H11.
+    rewrite /in_inset /inf lookup_insert /=. 
+    rewrite /default /id in H11.
+    destruct (lookup) eqn: Eqn.
+    + assert (dom (filter (λ '(k, _), (x < k)%Z) k) ⊆ dom k). { apply nzmap_dom_filter_subseteq. }
+      set_solver.
+    + rewrite /in_inset /inf Eqn /default in H4.
+      apply nzmap_elem_of_dom_total in H4.
+      rewrite nzmap_lookup_empty in H4. contradiction.
+  - intros.
+    destruct H11.
+    rewrite /in_inset /out /out_map /inf lookup_insert /= in H31. 
+    rewrite /in_outset /out /out_map nzmap_lookup_total_insert /inf.
+    destruct (lookup) eqn: Eqn.
+    simpl in H31.
+    rewrite /default /id.
+    admit.
+    set_solver.
+  - intros.
+    rewrite /in_outsets /in_outset /out /out_map /inf /= in H11. 
+    destruct H11 as (n1 & H11).
+    rewrite /in_outset /out /out_map nzmap_lookup_total_insert /inf.
+    destruct (decide (n1 = tp)).
+    { subst. rewrite nzmap_lookup_total_insert in H11. auto. }
+    { rewrite nzmap_lookup_total_insert_ne in H11. set_solver. auto. }
+  - simpl.
+    rewrite <- leibniz_equiv_iff.
+    rewrite nzmap_dom_insert_nonzero.
+    set_solver.
+    rewrite /out.
+    apply nzmap_elem_of_dom_total. rewrite H12. set_solver.
+  - rewrite /in_outset /out /= nzmap_lookup_total_insert in H11. 
+    specialize (H13 y).
+    apply H13 in H11. lia.
+  - rewrite /in_inset /inf lookup_insert. 
+    rewrite /in_outset /out nzmap_lookup_total_insert /= in H11. 
+    specialize (H13 y).
+    apply H13 in H11.
+    destruct H11.
+    assert ((x < y)%Z). lia.
+    destruct (lookup) eqn: Eqn.
+    rewrite /default /id.
+    admit.
+    rewrite /in_inset in H4.
+    rewrite /default /id.
+    rewrite /inf in H31. rewrite Eqn /= in H31. set_solver.
+  - intros.
+    destruct H11.
+    rewrite /in_inset /out /out_map /inf /= lookup_insert in H31. 
+    rewrite /in_outset /out nzmap_lookup_total_insert /=. 
+    apply H14.
+    exists n'. apply H13.
+    split; try done.
+    destruct (lookup) eqn: Eqn.
+    unfold inf.
+    rewrite Eqn /=.
+    assert (dom (filter (λ '(k, _), (x < k)%Z) k) ⊆ dom k). { apply nzmap_dom_filter_subseteq. }
+    set_solver.
+    apply nzmap_elem_of_dom_total in H31.
+    rewrite /in_inset /inf in H4.
+    rewrite Eqn in H4.
+    unfold default in H4. set_solver.
+  - intros.
+    rewrite /in_outsets /in_outset /out nzmap_lookup_total_insert /=.
+    apply H14.
+    rewrite /in_outsets /in_outset /out /= in H11. 
+    destruct H11 as (n1 & H11).
+    destruct (decide (n1 = n')) as [-> | Hn1n'].
+    { rewrite nzmap_lookup_total_insert in H11. by eexists. }
+    { rewrite nzmap_lookup_total_insert_ne in H11. by eexists. auto. }
+  - rewrite Hznth. entailer !.
+    iIntros "_".
+    iPureIntro.
+
+    
+    set I1 := flows.int
+       {|
+         infR := {[new_node := inf Ip tp]};
+         outR := <<[ tp := filter (λ '(k, _), (x < k)%Z) (inf Ip tp) ]>> ∅
+       |}.
+    set I2 := flows.int
+         {|
+           infR := {[tp := filter (λ '(k, _), (x < k)%Z) (inf Ip tp)]};
+           outR := <<[ n' := out Ip n' ]>> ∅
+         |}.
+
+    Check keyset _ _ Key I1 tp.
+    
+    
+    Admitted.
+
+
